tests/web_wasm/lean4lean_typechecker_shims.c
@@ -1,0 +1,22 @@
+typedef struct {
+    int      m_rc;
+    unsigned m_cs_sz:16;
+    unsigned m_other:8;
+    unsigned m_tag:8;
+} lean_object;
+
+extern lean_object *l_Lean_instInhabitedExpr;
+extern lean_object *lean_mk_string_from_bytes(const char *s, unsigned long sz);
+extern void *bump_alloc(unsigned long size);
+
+lean_object *_init_l_Lean_instInhabitedExpr(void) {
+    return l_Lean_instInhabitedExpr;
+}
+
+unsigned int lean4lean_alloc_bytes(unsigned int len) {
+    return (unsigned int)(unsigned long)bump_alloc((unsigned long)len);
+}
+
+lean_object *lean4lean_string_from_bytes(unsigned int ptr, unsigned int len) {
+    return lean_mk_string_from_bytes((const char *)(unsigned long)ptr, (unsigned long)len);
+}
